acorn-examples/Sorter.v
@@ -40,14 +40,13 @@ Section WithCava.
 Definition twoSorter {signal} `{Cava signal} {n}
                      (ab:  signal (Vec (Vec Bit n) 2)) :
                      cava (signal (Vec (Vec Bit n) 2)) :=
-   let a := indexConst ab 0 in
-   let b := indexConst ab 1 in
-   let comparison := greaterThanOrEqual (a, b) in
+   a <- indexConst ab 0 ;;
+   b <- indexConst ab 1 ;;
+   comparison <- greaterThanOrEqual (a, b) ;;
    negComparison <- inv comparison ;;
-   let sorted : Vector.t (signal (Vec Bit n)) 2 :=
-     [indexAt ab (unpeel [comparison]);
-      indexAt ab (unpeel [negComparison])] in
-   ret (unpeel sorted).
+   out0 <- indexAt ab (unpeel [comparison]) ;;
+   out1 <- indexAt ab (unpeel [negComparison]) ;;
+   ret (unpeel [out0;out1]).
 
 End WithCava.
 
