cava/Cava/Acorn/CombinationalProperties.v
@@ -154,12 +154,12 @@ Proof. destruct sel; reflexivity. Qed.
 Hint Rewrite @muxPair_correct using solve [eauto] : simpl_ident.
 
 Lemma indexAt2_correct {t} (i0 i1 : combType t) (sel : combType Bit) :
-  indexAt [i0; i1]%vector [sel]%vector = if sel then i1 else i0.
+  unIdent (indexAt [i0; i1]%vector [sel]%vector) = if sel then i1 else i0.
 Proof. destruct sel; reflexivity. Qed.
 Hint Rewrite @indexAt2_correct using solve [eauto] : simpl_ident.
 
 Lemma mux4_correct {t} (i0 i1 i2 i3 : combType t) (sel : combType (Vec Bit 2)) :
-  mux4 (i0,i1,i2,i3) sel =
+  unIdent (mux4 (i0,i1,i2,i3) sel) =
   if Vector.hd (Vector.tl sel)
   then if Vector.hd sel then i3 else i2
   else if Vector.hd sel then i1 else i0.
@@ -169,7 +169,7 @@ Qed.
 Hint Rewrite @mux4_correct using solve [eauto] : simpl_ident.
 
 Lemma indexConst_eq {A sz} (v : combType (Vec A sz)) (n : nat) :
-  indexConst v n = nth_default (defaultCombValue _) n v.
+  unIdent (indexConst v n) = nth_default (defaultCombValue _) n v.
 Proof. reflexivity. Qed.
 Hint Rewrite @indexConst_eq using solve [eauto] : simpl_ident.
 
